step nice, without code

EvmMachine.v
@@ -1,13 +1,95 @@
+(*
+Sources:
+"small ad-hoc symbolic interpreter" - https://gist.github.com/pirapira/0946d151e038393078c3
+CompCert - https://github.com/AbsInt/CompCert/blob/master/x86/Asm.v
+*)
+Require Import List.
+Require Import ZArith.
 
+Require Import Word.
+Require Import Instructions.
+Require Import Memory.
+Require Import Stack.
 
 Variable size : nat.
 
 Require Import Vector.
 Variable code : Vector.t instruction size.
+Variable jump_targets : list nat.
+
+
+Definition pc_t := Z.
+Definition inc_pc (pc : pc_t) : pc_t := Z.add pc (1%Z).
+Definition word_to_pc (w : word) : pc_t := Word.intval w.
+Definition pc_to_word (pc : pc_t) : word := Word.repr pc.
+
+Definition exec_jump_instr (i : instruction) (pc : pc_t) (ws : list word) : option (pc_t * list word) :=
+  match i with
+    | I_STOP => Some (pc, ws)
+    | I_JUMP => match ws with
+                  | (to::xs) => Some (word_to_pc to, xs)
+                  | _ => None
+                end
+    | I_JUMPI => match ws with
+                   | (to::cond::xs) => Some (if Word.eq cond Word.zero then (word_to_pc to) else (inc_pc pc), xs)
+                   | _ => None
+                end
+    | I_STACK_ONLY (I_PUSH _) => Some (inc_pc pc, ws) (* depends on code address encoding *)
+    | _ => Some (inc_pc pc, ws)
+  end.
+
 
 Record state := State {
   stack : list word;
-  mem  : memory;
+  mem : memory;
   stor : storage;
-  pc : nat;
+  pc : Z;
 }.
+
+Definition step (i : instruction) st m p pc : option state :=
+  let exec_so := fun i' => match exec_so_instr i' st with
+                             | Some st' => Some (State st' m p pc)
+                             | None => None
+                           end in
+  match i with
+  | I_STACK_ONLY i' => exec_so i'
+
+  | I_MEMINS i' => match exec_mem_instr i' m st with
+                     | Some (m', st') => Some (State st' m' p pc)
+                     | None => None
+                   end
+  | I_STORINS i' => match exec_storage_instr i' p st with
+                     | Some (p', st') => Some (State st' m p' pc)
+                     | None => None
+                   end
+
+  | I_STOP
+  | I_JUMP
+  | I_JUMPI => match exec_jump_instr i pc st with
+                 | Some (pc', st') => Some (State st' m p pc')
+                 | None => None
+               end
+  | I_PC => exec_so (I_PUSH (pc_to_word pc))
+  | I_OTHER _ => None
+  end.
+
+Ltac dis_invert e Q := destruct e; inversion Q; try reflexivity.
+
+Theorem step_nice : forall i st m p pc st' m' p' pc',
+  step i st m p pc = Some (State st' m' p' pc') ->
+    st' = firstn (alpha i) st' ++ skipn (delta i) st.
+Proof.
+  intros.
+  destruct i; simpl in H; inversion H; simpl; try reflexivity.
+  - apply exec_so_nice.
+    dis_invert (exec_so_instr s st) H.
+  - apply (exec_mem_nice _ m _ m' _).
+    dis_invert (exec_mem_instr m0 m st) H.
+    dis_invert p0 H.
+  - apply (exec_storage_nice _ p _ p' _).
+    dis_invert (exec_storage_instr s p st) H.
+    dis_invert p0 H.
+  - dis_invert st H.
+  - dis_invert st H.
+    dis_invert st H.
+Qed.
