Instructions.v
@@ -32,7 +32,6 @@ Inductive op3 : Type :=
 .
 
 Inductive so_instruction : Type :=
-  | I_STOP
   | I_OP1 : op1 -> so_instruction
   | I_OP2 : op2 -> so_instruction
   | I_OP3 : op3 -> so_instruction
@@ -53,31 +52,20 @@ Inductive storage_instruction : Type :=
   | I_SSTORE
 .
 
-Inductive instruction : Type :=
-  | I_STACK_ONLY : so_instruction -> instruction
+Inductive other_instruction : Type :=
   | I_SHA3
+  | I_ADDRESS | I_BALANCE | I_ORIGIN
+  | I_CALLER | I_CALLVALUE | I_CALLDATALOAD | I_CALLDATASIZE | I_CALLDATACOPY
+  | I_CODESIZE | I_CODECOPY | I_GASPRICE | I_EXTCODESIZE | I_EXTCODECOPY
+  | I_BLOCKHASH | I_COINBASE | I_TIMESTAMP | I_NUMBER | I_DIFFICULTY | I_GASLIMIT
+  | I_MSIZE | I_GAS | I_JUMPDEST (* NO-OP - mark as label *)
+  | I_LOG : nat (* 0-4 *) -> other_instruction
+  | I_CREATE | I_CALL | I_CALLCODE | I_RETURN | I_DELEGATECALL | I_SUICIDE
+.
 
-  | I_ADDRESS
-  | I_BALANCE
-  | I_ORIGIN
-  | I_CALLER
-  | I_CALLVALUE
-  | I_CALLDATALOAD
-  | I_CALLDATASIZE
-  | I_CALLDATACOPY
-  | I_CODESIZE
-  | I_CODECOPY
-  | I_GASPRICE
-  | I_EXTCODESIZE
-  | I_EXTCODECOPY
-
-  | I_BLOCKHASH
-  | I_COINBASE
-  | I_TIMESTAMP
-  | I_NUMBER
-  | I_DIFFICULTY
-  | I_GASLIMIT
-
+Inductive instruction : Type :=
+  | I_STOP
+  | I_STACK_ONLY : so_instruction -> instruction
   | I_MEMINS : mem_instruction -> instruction
   | I_STORINS : storage_instruction -> instruction
 
@@ -85,24 +73,13 @@ Inductive instruction : Type :=
   | I_JUMPI
   | I_PC
 
-  | I_MSIZE
-  | I_GAS
-  | I_JUMPDEST (* NO-OP - mark as label *)
-
-  | I_LOG : nat (* 0-4 *) -> instruction
-
-  | I_CREATE
-  | I_CALL
-  | I_CALLCODE
-  | I_RETURN
-  | I_DELEGATECALL
-  | I_SUICIDE
+  | I_OTHER : other_instruction -> instruction
 .
 
 
 Definition delta_alpha (i: instruction) : nat*nat :=
   match i with
-    | I_STACK_ONLY I_STOP => (0, 0)
+    | I_STOP => (0, 0)
     | I_STACK_ONLY (I_OP1 _) => (1, 1)
     | I_STACK_ONLY (I_OP2 _) => (2, 1)
     | I_STACK_ONLY (I_OP3 _) => (3, 1)
@@ -110,28 +87,28 @@ Definition delta_alpha (i: instruction) : nat*nat :=
     | I_STACK_ONLY (I_PUSH _) => (0, 1)
     | I_STACK_ONLY (I_DUP n _) => (1 + n, 2 + n)
     | I_STACK_ONLY (I_SWAP n _) => (2 + n, 2 + n)
-    | I_SHA3 => (2, 1)
+    | I_OTHER I_SHA3 => (2, 1)
 
-    | I_ADDRESS => (0, 1)
-    | I_BALANCE => (1, 1)
-    | I_ORIGIN => (0, 1)
-    | I_CALLER => (0, 1)
-    | I_CALLVALUE => (0, 1)
-    | I_CALLDATALOAD => (1, 1)
-    | I_CALLDATASIZE => (0, 1)
-    | I_CALLDATACOPY => (3, 0)
-    | I_CODESIZE => (0, 1)
-    | I_CODECOPY => (3, 0)
-    | I_GASPRICE => (0, 1)
-    | I_EXTCODESIZE => (1, 1)
-    | I_EXTCODECOPY => (4, 0)
+    | I_OTHER I_ADDRESS => (0, 1)
+    | I_OTHER I_BALANCE => (1, 1)
+    | I_OTHER I_ORIGIN => (0, 1)
+    | I_OTHER I_CALLER => (0, 1)
+    | I_OTHER I_CALLVALUE => (0, 1)
+    | I_OTHER I_CALLDATALOAD => (1, 1)
+    | I_OTHER I_CALLDATASIZE => (0, 1)
+    | I_OTHER I_CALLDATACOPY => (3, 0)
+    | I_OTHER I_CODESIZE => (0, 1)
+    | I_OTHER I_CODECOPY => (3, 0)
+    | I_OTHER I_GASPRICE => (0, 1)
+    | I_OTHER I_EXTCODESIZE => (1, 1)
+    | I_OTHER I_EXTCODECOPY => (4, 0)
 
-    | I_BLOCKHASH => (1, 1)
-    | I_COINBASE => (0, 1)
-    | I_TIMESTAMP => (0, 1)
-    | I_NUMBER => (0, 1)
-    | I_DIFFICULTY => (0, 1)
-    | I_GASLIMIT => (0, 1)
+    | I_OTHER I_BLOCKHASH => (1, 1)
+    | I_OTHER I_COINBASE => (0, 1)
+    | I_OTHER I_TIMESTAMP => (0, 1)
+    | I_OTHER I_NUMBER => (0, 1)
+    | I_OTHER I_DIFFICULTY => (0, 1)
+    | I_OTHER I_GASLIMIT => (0, 1)
 
     | I_MEMINS I_MLOAD => (1, 1)
     | I_MEMINS I_MSTORE => (2, 0)
@@ -143,18 +120,18 @@ Definition delta_alpha (i: instruction) : nat*nat :=
     | I_JUMPI => (2, 0)
     | I_PC => (0, 1)
 
-    | I_MSIZE => (0, 1)
-    | I_GAS => (0, 1)
-    | I_JUMPDEST  => (0, 0) (* NO-OP - mark as label *)
+    | I_OTHER I_MSIZE => (0, 1)
+    | I_OTHER I_GAS => (0, 1)
+    | I_OTHER I_JUMPDEST  => (0, 0) (* NO-OP - mark as label *)
 
-    | I_LOG n => (n + 2, 0)
+    | I_OTHER (I_LOG n) => (n + 2, 0)
 
-    | I_CREATE => (3, 1)
-    | I_CALL => (7, 1)
-    | I_CALLCODE => (7, 1)
-    | I_RETURN => (2, 0)
-    | I_DELEGATECALL => (6, 1)
-    | I_SUICIDE => (1, 10)
+    | I_OTHER I_CREATE => (3, 1)
+    | I_OTHER I_CALL => (7, 1)
+    | I_OTHER I_CALLCODE => (7, 1)
+    | I_OTHER I_RETURN => (2, 0)
+    | I_OTHER I_DELEGATECALL => (6, 1)
+    | I_OTHER I_SUICIDE => (1, 10)
   end.
 
 Definition delta (i: instruction) : nat := fst (delta_alpha i).
@@ -187,7 +164,7 @@ Definition eval_op2 (op : op2) (x y : word) : word :=
     | OP_AND => and x y
     | OP_OR => or x y
     | OP_XOR => xor x y
-    | OP_BYTE => least_byte x y
+    | OP_BYTE => get_byte x y
   end.
 
 Definition eval_op3 (op : op3) (x y m : word) : word :=
@@ -195,4 +172,3 @@ Definition eval_op3 (op : op3) (x y m : word) : word :=
     | OP_ADDMOD => addmod x y m
     | OP_MULMOD => mulmod x y m
   end.
-`
